I2SFI/AbstractMachine.v
@@ -1,0 +1,60 @@
+(**************************************************
+ * Author: Ana Nora Evans (ananevans@virginia.edu)
+ **************************************************)
+Require Import Coq.PArith.BinPos.
+
+Require Import Common.Definitions.
+
+Require Import Intermediate.Machine.
+Require Import TargetSFI.Machine.
+
+Definition label :Set := Component.id*positive.
+
+Definition register := RiscMachine.Register.t.
+
+Inductive ainstr :=
+| INop : ainstr
+| ILabel : label -> ainstr
+(* register operations *)
+| IConst : RiscMachine.value -> register -> ainstr
+| IMov : register -> register -> ainstr
+| IBinOp : RiscMachine.ISA.binop -> register -> register -> register -> ainstr
+(* memory operations *)
+| ILoad : register -> register -> ainstr
+| IStore : register -> register -> ainstr
+(* conditional and unconditional jumps *)
+| IBnz : register -> label -> ainstr
+| IJump : register -> ainstr
+| IJal : label -> ainstr
+(* termination *)
+| IHalt : ainstr.
+
+Definition code := list ainstr.
+
+Definition map_register (reg : Intermediate.Machine.register) : RiscMachine.Register.t :=
+  match reg with
+  | Intermediate.Machine.R_ONE => RiscMachine.Register.R_ONE
+  | Intermediate.Machine.R_COM => RiscMachine.Register.R_COM
+  | Intermediate.Machine.R_AUX1 => RiscMachine.Register.R_AUX1
+  | Intermediate.Machine.R_AUX2 => RiscMachine.Register.R_AUX2
+  | Intermediate.Machine.R_RA => RiscMachine.Register.R_RA
+  | Intermediate.Machine.R_SP => RiscMachine.Register.R_SP
+  end.
+
+Definition map_binop (op : Common.Values.binop) : RiscMachine.ISA.binop :=
+  match op with
+  | Add => RiscMachine.ISA.Addition
+  | Minus => RiscMachine.ISA.Subtraction
+  | Mul => RiscMachine.ISA.Multiplication
+  | Eq => RiscMachine.ISA.Equality
+  | Leq => RiscMachine.ISA.Leq
+  end.
+
+Record abstract_program :=
+  {
+    cn : Env.CN;
+    data_mem : RiscMachine.Memory.t;
+    prog_code : PMap.t (PMap.t code);
+    prog_interface : Program.interface;
+    prog_main : Component.id * Procedure.id
+  }.
