I2SFI/Compiler.v
@@ -1,0 +1,391 @@
+(**************************************************
+ * Author: Ana Nora Evans (ananevans@virginia.edu)
+ **************************************************)
+Require Import Coq.NArith.BinNat.
+Require Import Coq.Lists.List.
+Require Import Coq.Numbers.Natural.Peano.NPeano.
+
+Require Import Common.Maps.
+Require Import Common.Definitions.
+Require Import Intermediate.Machine.
+Require Import TargetSFI.Machine.
+Require Import I2SFI.CompMonad.
+Require Import I2SFI.AbstractMachine.
+
+Import MonadNotations.
+Open Scope monad_scope.
+
+Record compiler_env : Type := 
+  {
+    current_component : Component.id;
+    next_label : Intermediate.Machine.label;
+    cid2SFIid : PMap.t N;
+    (* intermediate component id -> block is -> sfi slot id *)
+    (* this is especially needed for static buffers *)
+    block_id2slot : PMap.t (PMap.t N)
+  }.
+
+Notation COMP := (Comp.t compiler_env).
+Notation get := (Comp.get compiler_env).
+Notation put := (Comp.put compiler_env).
+Notation modify := (Comp.modify compiler_env).
+Notation lift := (Comp.lift compiler_env).
+Notation fail := (Comp.fail compiler_env).
+Notation run := (Comp.run compiler_env).
+
+Definition gen_cn (pi : Program.interface) : list Component.id :=
+  List.map (fun '(key,_) => key) (PMap.elements pi).
+
+Definition with_current_component (cid : Component.id)
+           (env : compiler_env) :  compiler_env :=
+  {|
+    current_component := cid;
+    next_label := next_label env;
+    cid2SFIid := cid2SFIid env;
+    block_id2slot :=  block_id2slot env
+  |}.
+
+Definition env_add_blocks (cid : Component.id) (blocks : PMap.t N)
+           (env : compiler_env) :  compiler_env :=
+  {|
+    current_component := current_component env;
+    next_label := next_label env;
+    cid2SFIid := cid2SFIid env;
+    block_id2slot :=  PMap.add cid blocks (block_id2slot env)
+  |}.
+
+Definition with_fresh_label (lbl :  Intermediate.Machine.label)
+           (env : compiler_env) :  compiler_env :=
+   {|
+    current_component := current_component env;
+    block_id2slot :=  block_id2slot env;
+    cid2SFIid := cid2SFIid env;
+    next_label := (lbl + 1)%positive
+   |}.
+
+Definition with_cid2SFIid (m : PMap.t N)
+          (env : compiler_env) :  compiler_env :=
+  {|
+    current_component := current_component env;
+    next_label := next_label env;
+    block_id2slot := block_id2slot env;
+    cid2SFIid := m
+  |}.
+
+
+Definition gen_push_sfi (cid : Component.id) : AbstractMachine.code :=
+  [
+    AbstractMachine.IConst (RiscMachine.to_value (SFI.OFFSET_BITS_NO + SFI.COMP_BITS_NO + 1%N))
+                           RiscMachine.Register.R_AUX1
+    ; AbstractMachine.IBinOp (RiscMachine.ISA.ShiftLeft) RiscMachine.Register.R_AUX1
+                             RiscMachine.Register.R_SFI_SP RiscMachine.Register.R_AUX1
+    ; AbstractMachine.IBinOp (RiscMachine.ISA.BitwiseOr) RiscMachine.Register.R_AUX1
+                             RiscMachine.Register.R_OR_DATA_MASK RiscMachine.Register.R_AUX1
+    ; AbstractMachine.IStore RiscMachine.Register.R_AUX1 RiscMachine.Register.R_RA
+    ; AbstractMachine.IConst (1%Z) RiscMachine.Register.R_AUX1
+    ; AbstractMachine.IBinOp (RiscMachine.ISA.Addition) RiscMachine.Register.R_SFI_SP
+                             RiscMachine.Register.R_AUX1 RiscMachine.Register.R_SFI_SP
+  ]. 
+(* # form address (s=2*r_SFI_sp+1,c,o=0) in r₁ *)
+(*   Const r₁ <- N+S+1 *)
+(*   Binop r₁ <- r₁ SL r_SFI_sp  *)
+(*   Binop r₁ <- r₁ | r_or_data_mask *)
+(* # Store ra at the top of the stack *)
+(*   Store *r₁ <- ra *)
+(* # increment stack pointer *)
+(*   Const r₁ <- 1 *)
+(*   Binop r_SFI_sp <- r_SFI_sp + r₁  *)
+
+
+Definition gen_set_sfi_registers (cid : SFIComponent.id) : AbstractMachine.code :=
+  let data_mask := RiscMachine.to_value (SFI.or_data_mask cid) in
+  let code_mask := RiscMachine.to_value (SFI.or_code_mask cid) in
+  [
+      AbstractMachine.IConst data_mask RiscMachine.Register.R_OR_DATA_MASK
+    ; AbstractMachine.IConst code_mask RiscMachine.Register.R_OR_CODE_MASK
+    ; AbstractMachine.IConst data_mask RiscMachine.Register.R_D
+    ; AbstractMachine.IConst code_mask RiscMachine.Register.R_T
+  ].
+
+Definition get_address (cid : Component.id) (bid : Block.id)
+           (offset : Block.offset): COMP (RiscMachine.address) :=
+  do cenv <- get;
+    do cmap <- lift (PMap.find cid (block_id2slot cenv));
+    do slotid <- lift (PMap.find bid cmap);
+    if (Z.ltb offset 0%Z) then fail
+    else if (Z.leb (Z.of_N SFI.SLOT_SIZE) offset) then fail
+         else                                 
+           do sfiId <- lift (PMap.find cid (cid2SFIid cenv));
+           ret (SFI.address_of sfiId slotid (Z.to_N offset)).
+  
+
+Definition compile_IConst 
+           (imval : Intermediate.Machine.imvalue)
+           (reg : Intermediate.Machine.register)
+  : COMP (AbstractMachine.code) :=
+  let reg' := map_register reg in
+  match imval with
+  | Intermediate.Machine.IInt n => ret [AbstractMachine.IConst n reg']
+  | Intermediate.Machine.IPtr p =>
+    let cid := Pointer.component p in
+    let bid := Pointer.block p in
+    let offset := Pointer.offset p in
+    do address <- get_address cid bid offset;
+      ret  [AbstractMachine.IConst (RiscMachine.to_value address) reg']
+  end.
+
+Definition compile_IStore (rp : Intermediate.Machine.register)
+           (rs : Intermediate.Machine.register) : COMP (AbstractMachine.code) :=
+  ret [
+      AbstractMachine.IBinOp (RiscMachine.ISA.BitwiseAnd)
+                             (map_register rp) (RiscMachine.Register.R_AND_DATA_MASK)
+                             (RiscMachine.Register.R_D)
+      ; AbstractMachine.IBinOp (RiscMachine.ISA.BitwiseOr)
+                             (RiscMachine.Register.R_D) (RiscMachine.Register.R_OR_DATA_MASK)
+                             (RiscMachine.Register.R_D)
+      ; AbstractMachine.IStore (RiscMachine.Register.R_D) (map_register rs)
+    ].
+  (* Binop r_d <- r_p & r_and_data_mask  *)
+  (* Binop r_d <- r_d | r_or_data_mask(cid) *)
+  (* Store *r_d <- r_s *)
+
+(* TODO: Either use R_ONE or get rid of it *)
+Definition compile_IAlloc (rp : Intermediate.Machine.register)
+           (rs : Intermediate.Machine.register) : COMP (AbstractMachine.code) :=
+  do cenv <- get;
+    do cid <- lift (PMap.find (current_component cenv) (cid2SFIid cenv));
+    let rp' := (map_register rp) in
+    let rs' := (map_register rs) in
+    let (r1,r2) :=
+        if (RiscMachine.Register.eqb rp' rs')
+        then
+          if (RiscMachine.Register.eqb rp' RiscMachine.Register.R_AUX1)
+          then (RiscMachine.Register.R_AUX1,RiscMachine.Register.R_AUX2)
+          else (rp',RiscMachine.Register.R_AUX1)
+        else (rp',rs') in  ret
+    [
+    (* # save register r₂ at location (s=1,c,o=1) *)
+    (*   Const r₁ <- Address of (s=1,cid,o=1)  *)
+      AbstractMachine.IConst (RiscMachine.to_value (SFI.address_of cid 1%N 1%N))
+                             RiscMachine.Register.R_AUX1
+      (*   Store *r₁ <- r₂ *)
+      ; AbstractMachine.IStore RiscMachine.Register.R_AUX1 RiscMachine.Register.R_AUX2
+      (*   Const r₂ <- Address of (s=1,cid,o=0)  *)
+      ; AbstractMachine.IConst (RiscMachine.to_value (SFI.address_of cid 1%N 0%N))
+                             RiscMachine.Register.R_AUX2
+      (*   Load *r₂ -> r₁ *)
+      ; AbstractMachine.ILoad  RiscMachine.Register.R_AUX2  RiscMachine.Register.R_AUX1
+                             
+      (*   Const r₂ <- 1 *)
+      ; AbstractMachine.IConst (1%Z) RiscMachine.Register.R_AUX2
+
+      (*   Binop r₁ <- r₁ + r₂ *)
+      ; AbstractMachine.IBinOp (RiscMachine.ISA.Addition) RiscMachine.Register.R_AUX1
+                               RiscMachine.Register.R_AUX2 RiscMachine.Register.R_AUX1
+                             
+      (*   Const r₂ <- Address of (s=1,cid,o=0)  *)
+      ; AbstractMachine.IConst (RiscMachine.to_value (SFI.address_of cid 1%N 0%N))
+                             RiscMachine.Register.R_AUX2
+      (*   Store *r₂ <- r₁ *)
+      ; AbstractMachine.IStore RiscMachine.Register.R_AUX2 RiscMachine.Register.R_AUX1
+    
+      (*   Const r₂ <- 1 *)
+      ; AbstractMachine.IConst (1%Z) RiscMachine.Register.R_AUX2
+
+      (*   Binop r₁ <- r₁ - r₂ *)
+      ;  AbstractMachine.IBinOp (RiscMachine.ISA.Subtraction) RiscMachine.Register.R_AUX1
+                               RiscMachine.Register.R_AUX2 RiscMachine.Register.R_AUX1
+      (* # calculate address (s=2*k+1,c,o=0) in r₁ *)      
+      (*   Const r₂ <- N+S+1 *)
+      ; AbstractMachine.IConst (RiscMachine.to_value (SFI.OFFSET_BITS_NO + SFI.COMP_BITS_NO + 1%N))
+                           RiscMachine.Register.R_AUX2
+      (*   Binop r₁ <- r₁ << r₂ # k shift left (N+S+1) *)
+      ; AbstractMachine.IBinOp (RiscMachine.ISA.ShiftLeft) RiscMachine.Register.R_AUX1
+                             RiscMachine.Register.R_AUX2 RiscMachine.Register.R_AUX1
+      (*   Binop r₁ <- r₁ |  r_or_data_mask  *)
+      ;  AbstractMachine.IBinOp (RiscMachine.ISA.BitwiseOr) RiscMachine.Register.R_AUX1
+                             RiscMachine.Register.R_OR_DATA_MASK RiscMachine.Register.R_AUX1
+      (* # restore r₂ *)
+      (*   Const r₂ <- Address of (s=1,cid,o=1)  *)
+      ; AbstractMachine.IConst (RiscMachine.to_value (SFI.address_of cid 1%N 1%N))
+                               RiscMachine.Register.R_AUX1
+      (*   Load *r₂ -> r₂ *)
+      ;  AbstractMachine.ILoad  RiscMachine.Register.R_AUX2  RiscMachine.Register.R_AUX2
+                               
+  ]. 
+
+
+Definition compile_instruction 
+           (i : Intermediate.Machine.instr)
+  : COMP (AbstractMachine.code) :=
+  do cenv <- get;
+    let cid := (current_component cenv) in
+  match i with
+  | Intermediate.Machine.INop => ret [AbstractMachine.INop]
+  | Intermediate.Machine.ILabel lbl => ret [AbstractMachine.ILabel (cid,lbl)]
+  | Intermediate.Machine.IConst imval reg => (compile_IConst imval reg)
+  | Intermediate.Machine.IMov rs rd => ret [AbstractMachine.IMov
+                                             (map_register rs) (map_register rd)]
+  | Intermediate.Machine.IBinOp op r1 r2 rd => ret [AbstractMachine.IBinOp
+                                                     (map_binop op)
+                                                     (map_register r1) (map_register r2)
+                                                     (map_register rd)]
+  | Intermediate.Machine.ILoad rp rd => ret [AbstractMachine.ILoad (map_register rp)
+                                                                  (map_register rd)]
+  | Intermediate.Machine.IStore rp rs => (compile_IStore rp rs)
+  | Intermediate.Machine.IAlloc rp rs => (compile_IAlloc rp rs)
+  | Intermediate.Machine.IBnz r lbl => ret [AbstractMachine.IBnz (map_register r) (cid,lbl)]
+  | _ => ret [AbstractMachine.INop]
+  end.
+
+
+Fixpoint compile_instructions 
+         (ilist : Intermediate.Machine.code)
+  : COMP (AbstractMachine.code) :=
+  match (ilist) with
+  | [] => ret []
+  | i::xs =>
+    do ai <- compile_instruction i;
+    do res <- compile_instructions xs;
+    ret (ai ++ res)
+  end.
+
+Definition compile_procedure 
+           (pid : Procedure.id)
+           (code : Intermediate.Machine.code)
+           (interface : Program.interface) 
+  : COMP (AbstractMachine.code) :=
+  (* if the procedure is exported then must add the sfi stuff*)
+  do cenv <- get;
+    let cid := (current_component cenv) in
+    do comp_interface <- lift (PMap.find cid interface);
+    let proc_label := next_label cenv in
+    let exported_procs := Component.export comp_interface in
+    let is_exported := List.existsb (Pos.eqb pid) exported_procs in
+    do acode <- compile_instructions code;     
+      if is_exported then
+        do sfiId <- lift (PMap.find cid (cid2SFIid cenv));
+          ret (
+              [AbstractMachine.IHalt; AbstractMachine.ILabel (cid,proc_label)]
+                ++ (gen_push_sfi cid)
+                ++ (gen_set_sfi_registers sfiId)
+                ++ acode )
+      else
+        ret acode
+.
+
+Definition max_label (procs : list (Procedure.id * Intermediate.Machine.code))
+  : Intermediate.Machine.label :=
+  List.fold_left
+    Pos.max
+    (List.map
+       (fun i =>
+          match i with
+          | Intermediate.Machine.ILabel lbl => lbl
+          | _ => 1%positive (* impossible because of the filter *)
+          end
+       )
+       (List.filter (fun i =>
+                       match i with
+                       | Intermediate.Machine.ILabel _ => true
+                       | _ => false
+                       end
+                    )
+                    (List.flat_map snd procs)))
+    1%positive.
+
+Fixpoint compile_procedures (procs : list (Procedure.id * Intermediate.Machine.code))
+         (interface : Program.interface)
+  : COMP (list (Procedure.id * AbstractMachine.code)) :=
+  match procs with
+    | [] => ret []
+    | (pid,code) :: xs =>
+      do! modify (with_fresh_label (max_label procs));
+      do compiled_proc <- compile_procedure pid code interface;
+        do res <- compile_procedures xs interface;
+        ret ((pid, compiled_proc)::res)
+  end.
+  
+Fixpoint compile_components (components : list (Component.id * PMap.t Intermediate.Machine.code))
+         (interface : Program.interface)
+  : COMP (list (Component.id * PMap.t AbstractMachine.code)) :=
+  match components with
+  | [] => ret []
+  | (cid,procs)::xs =>
+    do! modify (with_current_component cid);
+    do procs <- compile_procedures (PMap.elements procs) interface;
+    do res <- compile_components xs interface;
+    ret ((cid, PMapExtra.of_list procs)::res)
+  end.
+  
+(* In slot 1 of each component store allocator data:
+for each component at address (s=1,cid,0) write number of buffers +1 
+*)
+Fixpoint allocate_buffers (buffs :  (list (Component.id * (list (Block.id * nat)))))
+           (cid2SFIid : PMap.t N) : COMP (RiscMachine.Memory.t) :=
+  match buffs with
+  | [] => ret RiscMachine.Memory.empty
+  | (cid,lst) :: xs =>
+    do mem <- allocate_buffers xs cid2SFIid;
+      match PMap.find cid cid2SFIid with
+      | None => fail
+      | Some sfi_cid =>
+        match List.find (fun '(_,size) => Nat.ltb (N.to_nat SFI.SLOT_SIZE) size) lst with
+        | None => 
+          let blocks := PMapExtra.of_list
+                          (List.combine (fst (List.split lst))
+                                        (SFI.Allocator.allocate_slots (List.length lst))) in
+          do! modify (env_add_blocks cid blocks); 
+            ret (RiscMachine.Memory.set_value
+                   mem
+                   (SFI.address_of sfi_cid (SFI.Allocator.allocator_data_slot) 0%N)
+                   (SFI.Allocator.initial_allocator_value (List.length lst)))
+        |_ => fail
+        end
+      end
+  end.
+
+Definition init_env : compiler_env :=
+  {| current_component := 1%positive;
+     next_label := 1%positive;
+     block_id2slot := PMap.empty (PMap.t N);
+     cid2SFIid := PMap.empty N
+  |}.
+
+Definition compile_abstract_program (ip : Intermediate.program) :
+  option (abstract_program) :=
+    (* cn maps sfi component id to intermediate component id *)
+    let cn := gen_cn (Intermediate.prog_interface ip) in
+    run init_env (
+          (* cid2SFIid maps intermediate component id to sfi id *)
+          let cid2SFIid := List.fold_left
+                             (fun acc '(cid,i)  =>
+                                PMap.add cid (Env.index2SFIid i) acc)
+                             (List.combine cn (List.seq 0 ((List.length cn) - 1)))
+                             (PMap.empty SFIComponent.id) in
+          do! modify (with_cid2SFIid cid2SFIid);
+          do mem <- allocate_buffers
+             (PMap.elements (Intermediate.prog_buffers ip))
+             cid2SFIid;
+            
+            do acode <- compile_components
+               (PMap.elements (Intermediate.prog_procedures ip) )
+               (Intermediate.prog_interface ip);
+
+            ret {| AbstractMachine.cn := cn;
+                   data_mem := mem;
+                   prog_code := PMapExtra.of_list acode;
+                   AbstractMachine.prog_interface := Intermediate.prog_interface ip;
+                   AbstractMachine.prog_main := Intermediate.prog_main ip
+                |}
+            
+    ).
+
+Definition compile_program (ip : Intermediate.program) :
+  option (sfi_program) := None.
+(* layout code in memory *)
+(* replace labels with addresses *)
+              (* generate code for component 0
+       push address of halt on sfi stack
+       call main === changes mem *)
+(* generate E *)
